theories/rule_base.v
@@ -1,6 +1,44 @@
 From iris.algebra Require Import gmap gset.
 From HypVeri Require Import RAs.
 
+  Lemma option_state_unpack_preserve_state_Some σ1 σ2 σ2' :
+   σ2' = Some σ2 ->  (ExecI, σ2) = (option_state_unpack σ1 σ2').
+  Proof.
+    intros.
+    destruct σ2' eqn:Heqn.
+    inversion H; subst.
+    done.
+    done.
+  Qed.
+
+
+  Lemma mov_word_ExecI σ1 r w :
+   PC ≠ r ->  NZ ≠ r -> (mov_word σ1 r w)= (ExecI, (update_incr_PC (update_reg σ1 r w))).
+  Proof.
+    intros.
+    unfold mov_word .
+    destruct r;[contradiction|contradiction|].
+    rewrite <- (option_state_unpack_preserve_state_Some σ1
+                                                        (update_incr_PC (update_reg σ1 (R n fin) w)) (Some (update_incr_PC (update_reg σ1 (R n fin) w))));eauto.
+  Qed.
+
+
+
+  Lemma update_reg_global_preserve_current_vm σ r w :(get_current_vm (update_reg_global σ (get_current_vm σ) r w)) = (get_current_vm σ).
+  Proof.
+    unfold get_current_vm ,update_reg_global.
+    simpl.
+    unfold get_current_vm.
+    reflexivity.
+  Qed.
+
+  Lemma update_offset_PC_preserve_current_vm σ d o :(get_current_vm (update_offset_PC σ d o )) = (get_current_vm σ).
+  Proof.
+    unfold get_current_vm ,update_offset_PC.
+    unfold get_current_vm.
+    destruct (get_vm_reg_file σ σ.1.1.2 !! PC),d;eauto.
+  Qed.
+
   Lemma get_reg_gmap_lookup_Some σ i r w : (get_reg_gmap σ) !! (r,i)= Some w <->  get_vm_reg_file σ i !! r = Some w.
     Proof.
       split.
@@ -174,7 +212,30 @@ From HypVeri Require Import RAs.
     by rewrite H4.
   Qed.
 
-   Lemma update_reg_global_preserve_tx σ i r w : get_tx_agree (update_reg_global σ i r w) =
+  Lemma update_reg_global_preserve_mem σ i r w : get_mem (update_reg_global σ i r w) = get_mem σ.
+  Proof.
+    unfold update_reg_global, get_mem.
+    simpl.
+    reflexivity.
+  Qed.
+
+  Lemma update_reg_preserve_mem σ r w : get_mem (update_reg σ r w) = get_mem σ.
+  Proof.
+    unfold update_reg.
+    apply update_reg_global_preserve_mem.
+  Qed.
+
+  Lemma update_offset_PC_preserve_mem σ d o : get_mem (update_offset_PC σ d o) = get_mem σ.
+  Proof.
+    unfold update_offset_PC.
+
+    destruct (get_vm_reg_file σ (get_current_vm σ) !! PC).
+    destruct d; rewrite -> update_reg_preserve_mem;done.
+    done.
+  Qed.
+
+
+  Lemma update_reg_global_preserve_tx σ i r w : get_tx_agree (update_reg_global σ i r w) =
                                                (get_tx_agree σ).
   Proof.
     rewrite /get_tx_agree /get_txrx_auth_agree.
